driver/ParallelPolOpt.v
@@ -6,6 +6,7 @@ Require Import OpenScop.
 Require Import ParallelCodegen.
 Require Import Validator.
 Require Import PolOpt.
+Require Import TilingBandScheduleValidator.
 Require Import ImpureAlarmConfig.
 Require Import Vpl.Impure.
 
@@ -16,6 +17,7 @@ Module PolyLang := PolIRs.PolyLang.
 Module State := PolIRs.State.
 Module ValidatorCore := Validator PolIRs.
 Module ParallelCodegenCore := ParallelCodegen PolIRs.
+Module TilingSched := TilingBandScheduleValidator PolIRs.
 Module LoopIR := PolIRs.Loop.
 
 Definition parallel_plan_of_dim (d : nat) : ValidatorCore.parallel_plan :=
@@ -92,6 +94,78 @@ Definition try_phase_pipeline_from_source_pol_poly
           BIND affine_ok <- ValidatorCore.validate pol_source pol_mid -;
           if affine_ok then
             try_verified_tiling_after_phase_mid_poly pol_mid mid_scop after_scop
+          else
+            CoreOpt.checked_affine_schedule pol_source
+      end
+  end.
+
+Definition try_verified_diamond_after_phase_mid_poly
+    (pol_mid : PolyLang.t)
+    (mid_scop posttile_scop after_scop : OpenScop)
+  : imp PolyLang.t :=
+  match CoreOpt.infer_tiling_witness_scops mid_scop posttile_scop with
+  | Err _ =>
+      pure pol_mid
+  | Okk ws =>
+      match ValidatorCore.import_canonical_tiled_after_poly pol_mid posttile_scop ws with
+      | Err _ =>
+          pure pol_mid
+      | Okk pol_posttile =>
+          BIND ok_shape <- TilingSched.checked_tiling_schedule_stripmined_validate_poly pol_mid pol_posttile ws -;
+          if ok_shape then
+            match TilingSched.infer_pprog_tiling_bands
+                    (TilingSched.Base.outer_to_tiling_pprog pol_mid) ws with
+            | None =>
+                pure pol_mid
+            | Some bands =>
+                BIND ok_perm <-
+                  TilingSched.check_pprog_permutable_tiling_bands_via_validate_tiling
+                    (TilingSched.Base.outer_to_tiling_pprog pol_mid)
+                    (TilingSched.Base.outer_to_tiling_pprog pol_posttile)
+                    ws bands -;
+                if ok_perm then
+                  BIND wf_posttile <- ValidatorCore.check_wf_polyprog_general pol_posttile -;
+                  if wf_posttile then
+                    match PolyLang.from_openscop_schedule_only pol_posttile after_scop with
+                    | Err _ =>
+                        pure pol_mid
+                    | Okk pol_after =>
+                        BIND final_ok <- ValidatorCore.validate_general pol_posttile pol_after -;
+                        if final_ok then
+                          BIND wf_after <- ValidatorCore.check_wf_polyprog_general pol_after -;
+                          if wf_after then
+                            pure (PolyLang.current_view_pprog pol_after)
+                          else
+                            pure pol_mid
+                        else
+                          pure pol_mid
+                    end
+                  else
+                    pure pol_mid
+                else
+                  pure pol_mid
+            end
+          else
+            pure pol_mid
+      end
+  end.
+
+Definition try_diamond_phase_pipeline_from_source_pol_poly
+    (pol_source : PolyLang.t)
+    (before_scop : OpenScop)
+  : imp PolyLang.t :=
+  match CoreOpt.run_pluto_diamond_phase_pipeline before_scop with
+  | Err _ =>
+      CoreOpt.checked_affine_schedule pol_source
+  | Okk (mid_scop, (posttile_scop, after_scop)) =>
+      match PolyLang.from_openscop_like_source pol_source mid_scop with
+      | Err _ =>
+          CoreOpt.checked_affine_schedule pol_source
+      | Okk pol_mid =>
+          BIND affine_ok <- ValidatorCore.validate pol_source pol_mid -;
+          if affine_ok then
+            try_verified_diamond_after_phase_mid_poly
+              pol_mid mid_scop posttile_scop after_scop
           else
             CoreOpt.checked_affine_schedule pol_source
       end
@@ -181,11 +255,31 @@ Definition phase_pipeline_opt_prepared_from_poly_with_iss_poly
   else
     pure pol.
 
+Definition diamond_phase_pipeline_opt_prepared_from_poly_no_iss_poly
+    (pol : PolyLang.t)
+  : imp PolyLang.t :=
+  if CoreOpt.has_nonscalar_stmt pol then
+    match CoreOpt.export_for_phase_scheduler pol with
+    | None =>
+        CoreOpt.checked_affine_schedule pol
+    | Some before_scop =>
+        try_diamond_phase_pipeline_from_source_pol_poly pol before_scop
+    end
+  else
+    pure pol.
+
 Definition parallel_current_prepared_from_poly
     (pol : PolyLang.t)
     (d : nat)
   : imp (result ParallelCodegenCore.ParallelLoop.t) :=
   BIND pol' <- phase_pipeline_opt_prepared_from_poly_no_iss_poly pol -;
+  checked_parallel_current_annotated_codegen_at pol' d.
+
+Definition parallel_current_diamond_prepared_from_poly
+    (pol : PolyLang.t)
+    (d : nat)
+  : imp (result ParallelCodegenCore.ParallelLoop.t) :=
+  BIND pol' <- diamond_phase_pipeline_opt_prepared_from_poly_no_iss_poly pol -;
   checked_parallel_current_annotated_codegen_at pol' d.
 
 Definition parallel_current_identity_prepared_from_poly_with_iss
@@ -236,6 +330,14 @@ Definition Opt_parallel_current_result
   let pol := CoreOpt.Strengthen.strengthen_pprog pol0 in
   parallel_current_prepared_from_poly pol d.
 
+Definition Opt_parallel_current_diamond_result
+    (loop : LoopIR.t)
+    (d : nat)
+  : imp (result ParallelCodegenCore.ParallelLoop.t) :=
+  BIND pol0 <- res_to_alarm PolyLang.dummy (CoreOpt.Extractor.extractor loop) -;
+  let pol := CoreOpt.Strengthen.strengthen_pprog pol0 in
+  parallel_current_diamond_prepared_from_poly pol d.
+
 Definition Opt_parallel_current_identity_with_iss_result
     (loop : LoopIR.t)
     (d : nat)
@@ -279,6 +381,13 @@ Definition Opt_parallel_current
     (d : nat)
   : imp ParallelCodegenCore.ParallelLoop.t :=
   BIND res <- Opt_parallel_current_result loop d -;
+  res_to_alarm parallel_dummy res.
+
+Definition Opt_parallel_current_diamond
+    (loop : LoopIR.t)
+    (d : nat)
+  : imp ParallelCodegenCore.ParallelLoop.t :=
+  BIND res <- Opt_parallel_current_diamond_result loop d -;
   res_to_alarm parallel_dummy res.
 
 Definition Opt_parallel_current_identity_with_iss
