driver/PolOptBandTiling.v
@@ -4,6 +4,7 @@ Require Import PolIRs.
 Require Import OpenScop.
 Require Import Result.
 Require Import PolOpt.
+Require Import ISSValidatorCorrect.
 Require Import ImpureAlarmConfig.
 Require Import Vpl.Impure.
 
@@ -13,6 +14,7 @@ Module BaseOpt := PolOpt PolIRs.
 Module ValidatorCore := BaseOpt.ValidatorCore.
 Module PrepareCore := BaseOpt.PrepareCore.
 Module TilingSched := TilingBandScheduleValidator PolIRs.
+Module ISSValidatorCorrectCore := ISSValidatorCorrect PolIRs.
 Module PolyLang := PolIRs.PolyLang.
 Module LoopIR := PolIRs.Loop.
 Module State := PolIRs.State.
@@ -148,6 +150,44 @@ Definition try_diamond_phase_pipeline_from_source_pol_band
       end
   end.
 
+Definition try_diamond_phase_pipeline_from_source_pol_band_with_iss
+    (pol_source: PolyLang.t)
+    (before_scop: OpenScop): imp LoopIR.t :=
+  match BaseOpt.run_pluto_diamond_phase_pipeline_with_iss before_scop with
+  | Err _ =>
+      BaseOpt.affine_only_opt_prepared_from_poly pol_source
+  | Okk (mid_scop, (posttile_scop, after_scop)) =>
+      match PolyLang.from_openscop_like_source pol_source mid_scop with
+      | Err _ =>
+          BaseOpt.affine_only_opt_prepared_from_poly pol_source
+      | Okk pol_mid =>
+          BIND affine_ok <- ValidatorCore.validate pol_source pol_mid -;
+          if affine_ok then
+            try_verified_diamond_after_phase_mid_band
+              pol_mid mid_scop posttile_scop after_scop
+          else
+            BaseOpt.affine_only_opt_prepared_from_poly pol_source
+      end
+  end.
+
+Definition try_checked_iss_diamond_phase_pipeline_from_poly_band
+    (pol: PolyLang.t)
+    (before_scop: OpenScop): imp LoopIR.t :=
+  match BaseOpt.infer_iss_from_source_scop pol before_scop with
+  | Okk (Some (pol_iss, w)) =>
+      if ValidatorCore.checked_iss_complete_cut_shape_validate pol pol_iss w then
+        BIND iss_wf <- ValidatorCore.check_wf_polyprog pol_iss -;
+        if iss_wf then
+          try_diamond_phase_pipeline_from_source_pol_band_with_iss
+            pol_iss before_scop
+        else
+          try_diamond_phase_pipeline_from_source_pol_band pol before_scop
+      else
+        try_diamond_phase_pipeline_from_source_pol_band pol before_scop
+  | _ =>
+      try_diamond_phase_pipeline_from_source_pol_band pol before_scop
+  end.
+
 Definition phase_pipeline_opt_prepared_from_poly_no_iss_band
     (pol: PolyLang.t): imp LoopIR.t :=
   if BaseOpt.has_nonscalar_stmt pol then
@@ -175,6 +215,18 @@ Definition phase_diamond_opt_prepared_from_poly_no_iss_band
   else
     PrepareCore.prepared_codegen pol.
 
+Definition phase_diamond_opt_prepared_from_poly_with_iss_band
+    (pol: PolyLang.t): imp LoopIR.t :=
+  if BaseOpt.has_nonscalar_stmt pol then
+    match BaseOpt.export_for_phase_scheduler pol with
+    | Some before_scop =>
+        try_checked_iss_diamond_phase_pipeline_from_poly_band pol before_scop
+    | None =>
+        BaseOpt.affine_only_opt_prepared_from_poly pol
+    end
+  else
+    PrepareCore.prepared_codegen pol.
+
 Definition phase_pipeline_opt_prepared_band
     (loop: LoopIR.t): imp LoopIR.t :=
   BIND pol0 <- res_to_alarm PolyLang.dummy (BaseOpt.Extractor.extractor loop) -;
@@ -186,6 +238,12 @@ Definition phase_diamond_opt_prepared_band
   BIND pol0 <- res_to_alarm PolyLang.dummy (BaseOpt.Extractor.extractor loop) -;
   let pol := BaseOpt.Strengthen.strengthen_pprog pol0 in
   phase_diamond_opt_prepared_from_poly_no_iss_band pol.
+
+Definition phase_diamond_opt_prepared_with_iss_band
+    (loop: LoopIR.t): imp LoopIR.t :=
+  BIND pol0 <- res_to_alarm PolyLang.dummy (BaseOpt.Extractor.extractor loop) -;
+  let pol := BaseOpt.Strengthen.strengthen_pprog pol0 in
+  phase_diamond_opt_prepared_from_poly_with_iss_band pol.
 
 Lemma try_verified_tiling_after_phase_mid_band_correct:
   forall pol_mid mid_scop after_scop st st',
@@ -656,6 +714,92 @@ Proof.
   - eapply BaseOpt.affine_opt_prepared_from_poly_correct; eauto.
 Qed.
 
+Lemma try_diamond_phase_pipeline_from_source_pol_band_with_iss_correct:
+  forall pol_source before_scop st st',
+    PolyLang.wf_pprog_affine pol_source ->
+    WHEN loop' <-
+      try_diamond_phase_pipeline_from_source_pol_band_with_iss
+        pol_source before_scop THEN
+    LoopIR.semantics loop' st st' ->
+    exists st'',
+      PolyLang.instance_list_semantics pol_source st st'' /\
+      State.eq st' st''.
+Proof.
+  intros pol_source before_scop st st' Hwf_source loop' Hopt Hloop.
+  unfold try_diamond_phase_pipeline_from_source_pol_band_with_iss in Hopt.
+  destruct (BaseOpt.run_pluto_diamond_phase_pipeline_with_iss before_scop)
+    as [[mid_scop [posttile_scop after_scop]]|msg] eqn:Hphase.
+  - destruct (PolyLang.from_openscop_like_source pol_source mid_scop)
+      as [pol_mid|msg_mid] eqn:Hmid.
+    + bind_imp_destruct Hopt affine_ok Haff.
+      destruct affine_ok.
+      * pose proof
+          (ValidatorCore.validate_preserve_wf_pprog
+             pol_source pol_mid _ Haff eq_refl)
+          as [_ Hwf_mid].
+        pose proof
+          (try_verified_diamond_after_phase_mid_band_correct
+             pol_mid mid_scop posttile_scop after_scop
+             st st' Hwf_mid loop' Hopt Hloop)
+          as Hmid_corr.
+        destruct Hmid_corr as [st_mid [Hmid_sem Heq_mid]].
+        pose proof
+          (ValidatorCore.validate_correct
+             pol_source pol_mid st st_mid true Haff eq_refl Hmid_sem)
+          as Haff_corr.
+        destruct Haff_corr as [st_src [Hsrc_sem Heq_src]].
+        exists st_src.
+        split; auto.
+        eapply State.eq_trans; eauto.
+      * eapply BaseOpt.affine_opt_prepared_from_poly_correct; eauto.
+    + eapply BaseOpt.affine_opt_prepared_from_poly_correct; eauto.
+  - eapply BaseOpt.affine_opt_prepared_from_poly_correct; eauto.
+Qed.
+
+Lemma try_checked_iss_diamond_phase_pipeline_from_poly_band_correct:
+  forall pol before_scop st st',
+    PolyLang.wf_pprog_affine pol ->
+    WHEN loop' <-
+      try_checked_iss_diamond_phase_pipeline_from_poly_band
+        pol before_scop THEN
+    LoopIR.semantics loop' st st' ->
+    exists st'',
+      PolyLang.instance_list_semantics pol st st'' /\
+      State.eq st' st''.
+Proof.
+  intros pol before_scop st st' Hwf loop' Hopt Hloop.
+  unfold try_checked_iss_diamond_phase_pipeline_from_poly_band in Hopt.
+  destruct (BaseOpt.infer_iss_from_source_scop pol before_scop) as [iss_opt|msg]
+    eqn:Hiss_infer.
+  - destruct iss_opt as [[pol_iss w]|].
+    + destruct (ValidatorCore.checked_iss_complete_cut_shape_validate pol pol_iss w)
+        eqn:Hiss_check.
+      * bind_imp_destruct Hopt iss_wf Hiss_wf.
+        destruct iss_wf.
+        -- pose proof
+             (BaseOpt.check_wf_polyprog_affine_correct
+                pol_iss _ Hiss_wf eq_refl)
+             as Hwf_iss.
+           pose proof
+             (try_diamond_phase_pipeline_from_source_pol_band_with_iss_correct
+                pol_iss before_scop st st' Hwf_iss loop' Hopt Hloop)
+             as Hiss_corr.
+           destruct Hiss_corr as [st_iss [Hiss_sem Heq_iss]].
+           pose proof
+             (ISSValidatorCorrectCore
+                .checked_iss_complete_cut_shape_validate_semantics_correct
+                pol pol_iss w st st_iss Hiss_check Hiss_sem)
+             as Hback.
+           destruct Hback as [st_src [Hsrc_sem Heq_src]].
+           exists st_src.
+           split; auto.
+           eapply State.eq_trans; eauto.
+        -- eapply try_diamond_phase_pipeline_from_source_pol_band_correct; eauto.
+      * eapply try_diamond_phase_pipeline_from_source_pol_band_correct; eauto.
+    + eapply try_diamond_phase_pipeline_from_source_pol_band_correct; eauto.
+  - eapply try_diamond_phase_pipeline_from_source_pol_band_correct; eauto.
+Qed.
+
 Lemma phase_diamond_opt_prepared_from_poly_no_iss_band_correct:
   forall pol st st',
     PolyLang.wf_pprog_affine pol ->
@@ -678,8 +822,33 @@ Proof.
     exists st'. split; auto. apply State.eq_refl.
 Qed.
 
+Lemma phase_diamond_opt_prepared_from_poly_with_iss_band_correct:
+  forall pol st st',
+    PolyLang.wf_pprog_affine pol ->
+    WHEN loop' <- phase_diamond_opt_prepared_from_poly_with_iss_band pol THEN
+    LoopIR.semantics loop' st st' ->
+    exists st'',
+      PolyLang.instance_list_semantics pol st st'' /\
+      State.eq st' st''.
+Proof.
+  intros pol st st' Hwf loop' Hopt Hloop.
+  unfold phase_diamond_opt_prepared_from_poly_with_iss_band in Hopt.
+  destruct (BaseOpt.has_nonscalar_stmt pol) eqn:Hnonscalar.
+  - destruct (BaseOpt.export_for_phase_scheduler pol) as [before_scop|] eqn:Hscop.
+    + eapply try_checked_iss_diamond_phase_pipeline_from_poly_band_correct; eauto.
+    + eapply BaseOpt.affine_opt_prepared_from_poly_correct; eauto.
+  - pose proof
+      (PrepareCore.prepared_codegen_correct
+         pol st st' loop' Hopt Hwf Hloop)
+      as Hsem.
+    exists st'. split; auto. apply State.eq_refl.
+Qed.
+
 Definition Opt_prepared_diamond_band := phase_diamond_opt_prepared_band.
 Definition Opt_diamond_band := Opt_prepared_diamond_band.
+Definition Opt_prepared_diamond_band_with_iss :=
+  phase_diamond_opt_prepared_with_iss_band.
+Definition Opt_diamond_band_with_iss := Opt_prepared_diamond_band_with_iss.
 
 Theorem Opt_prepared_diamond_band_correct:
   forall loop st st',
@@ -726,6 +895,54 @@ Theorem Opt_diamond_band_correct:
 Proof.
   intros.
   eapply Opt_prepared_diamond_band_correct; eauto.
+Qed.
+
+Theorem Opt_prepared_diamond_band_with_iss_correct:
+  forall loop st st',
+    WHEN loop' <- Opt_prepared_diamond_band_with_iss loop THEN
+    LoopIR.semantics loop' st st' ->
+    exists st'',
+      LoopIR.semantics loop st st'' /\
+      State.eq st' st''.
+Proof.
+  intros loop st st' loop' Hopt Hloop.
+  unfold Opt_prepared_diamond_band_with_iss,
+    phase_diamond_opt_prepared_with_iss_band in Hopt.
+  bind_imp_destruct Hopt pol0 Hextimp.
+  set (pol := BaseOpt.Strengthen.strengthen_pprog pol0) in *.
+  pose proof Hextimp as Hextok.
+  apply res_to_alarm_correct in Hextok.
+  pose proof
+    (BaseOpt.Strengthen.strengthen_pprog_wf_affine pol0
+       (BaseOpt.extractor_success_wf_pprog_affine loop pol0 Hextok))
+    as Hwf_pol.
+  pose proof
+    (phase_diamond_opt_prepared_from_poly_with_iss_band_correct
+       pol st st' Hwf_pol loop' Hopt Hloop)
+    as Hphase_corr.
+  destruct Hphase_corr as [st_str [Hstr_sem Heq_str]].
+  eapply BaseOpt.Strengthen.instance_list_semantics_unstrengthen in Hstr_sem.
+  pose proof
+    (BaseOpt.Extractor.extractor_correct loop pol0 st st_str Hextok Hstr_sem)
+    as Hext_corr.
+  destruct Hext_corr as [st_src [Hloop_src Heq_src]].
+  exists st_src.
+  split; auto.
+  eapply State.eq_trans.
+  - exact Heq_str.
+  - exact Heq_src.
+Qed.
+
+Theorem Opt_diamond_band_with_iss_correct:
+  forall loop st st',
+    WHEN loop' <- Opt_diamond_band_with_iss loop THEN
+    LoopIR.semantics loop' st st' ->
+    exists st'',
+      LoopIR.semantics loop st st'' /\
+      State.eq st' st''.
+Proof.
+  intros.
+  eapply Opt_prepared_diamond_band_with_iss_correct; eauto.
 Qed.
 
 Theorem Opt_band_correct:
