src/TPolIRs.v
@@ -24,6 +24,8 @@ Module TPolIRs <: POLIRS with Module Instr := TInstr.
      OpenScop -> result (OpenScop * OpenScop).
    Parameter diamond_phase_scop_scheduler :
      OpenScop -> result (OpenScop * (OpenScop * OpenScop)).
+   Parameter diamond_phase_scop_scheduler_with_iss :
+     OpenScop -> result (OpenScop * (OpenScop * OpenScop)).
    Parameter infer_iss_from_source_scop :
      PolyLang.t -> OpenScop -> result (option (PolyLang.t * iss_witness)).
    Parameter infer_tiling_witness_scops:
@@ -50,4 +52,6 @@ Module TPolIRs <: POLIRS with Module Instr := TInstr.
      phase_scop_scheduler_with_iss.
    Definition run_pluto_diamond_phase_pipeline :=
      diamond_phase_scop_scheduler.
+   Definition run_pluto_diamond_phase_pipeline_with_iss :=
+     diamond_phase_scop_scheduler_with_iss.
 End TPolIRs.
