syntax/SParallelPolOpt.v
@@ -5,6 +5,7 @@ Require Import OpenScop.
 Require Import ParallelCodegen.
 Require Import Validator.
 Require Import PolOpt.
+Require Import STilingBandSched.
 Require Import ImpureAlarmConfig.
 Require Import Vpl.Impure.
 
@@ -94,6 +95,78 @@ Definition try_phase_pipeline_from_source_pol_poly
       end
   end.
 
+Definition try_verified_diamond_after_phase_mid_poly
+    (pol_mid : PolyLang.t)
+    (mid_scop posttile_scop after_scop : OpenScop)
+  : imp PolyLang.t :=
+  match CoreOpt.infer_tiling_witness_scops mid_scop posttile_scop with
+  | Err _ =>
+      pure pol_mid
+  | Okk ws =>
+      match ValidatorCore.import_canonical_tiled_after_poly pol_mid posttile_scop ws with
+      | Err _ =>
+          pure pol_mid
+      | Okk pol_posttile =>
+          BIND ok_shape <- STilingBandSched.checked_tiling_schedule_stripmined_validate_poly pol_mid pol_posttile ws -;
+          if ok_shape then
+            match STilingBandSched.infer_pprog_tiling_bands
+                    (STilingBandSched.outer_to_tiling_pprog pol_mid) ws with
+            | None =>
+                pure pol_mid
+            | Some bands =>
+                BIND ok_perm <-
+                  STilingBandSched.check_pprog_permutable_tiling_bands
+                    (STilingBandSched.outer_to_tiling_pprog pol_mid)
+                    (STilingBandSched.outer_to_tiling_pprog pol_posttile)
+                    ws bands -;
+                if ok_perm then
+                  BIND wf_posttile <- ValidatorCore.check_wf_polyprog_general pol_posttile -;
+                  if wf_posttile then
+                    match PolyLang.from_openscop_schedule_only pol_posttile after_scop with
+                    | Err _ =>
+                        pure pol_mid
+                    | Okk pol_after =>
+                        BIND final_ok <- ValidatorCore.validate_general pol_posttile pol_after -;
+                        if final_ok then
+                          BIND wf_after <- ValidatorCore.check_wf_polyprog_general pol_after -;
+                          if wf_after then
+                            pure (PolyLang.current_view_pprog pol_after)
+                          else
+                            pure pol_mid
+                        else
+                          pure pol_mid
+                    end
+                  else
+                    pure pol_mid
+                else
+                  pure pol_mid
+            end
+          else
+            pure pol_mid
+      end
+  end.
+
+Definition try_diamond_phase_pipeline_from_source_pol_poly
+    (pol_source : PolyLang.t)
+    (before_scop : OpenScop)
+  : imp PolyLang.t :=
+  match CoreOpt.run_pluto_diamond_phase_pipeline before_scop with
+  | Err _ =>
+      CoreOpt.checked_affine_schedule pol_source
+  | Okk (mid_scop, (posttile_scop, after_scop)) =>
+      match PolyLang.from_openscop_like_source pol_source mid_scop with
+      | Err _ =>
+          CoreOpt.checked_affine_schedule pol_source
+      | Okk pol_mid =>
+          BIND affine_ok <- ValidatorCore.validate pol_source pol_mid -;
+          if affine_ok then
+            try_verified_diamond_after_phase_mid_poly
+              pol_mid mid_scop posttile_scop after_scop
+          else
+            CoreOpt.checked_affine_schedule pol_source
+      end
+  end.
+
 Definition try_checked_iss_phase_pipeline_from_poly_poly
     (pol : PolyLang.t)
     (before_scop : OpenScop)
@@ -178,11 +251,31 @@ Definition phase_pipeline_opt_prepared_from_poly_with_iss_poly
   else
     pure pol.
 
+Definition diamond_phase_pipeline_opt_prepared_from_poly_no_iss_poly
+    (pol : PolyLang.t)
+  : imp PolyLang.t :=
+  if CoreOpt.has_nonscalar_stmt pol then
+    match CoreOpt.export_for_phase_scheduler pol with
+    | None =>
+        CoreOpt.checked_affine_schedule pol
+    | Some before_scop =>
+        try_diamond_phase_pipeline_from_source_pol_poly pol before_scop
+    end
+  else
+    pure pol.
+
 Definition parallel_current_prepared_from_poly
     (pol : PolyLang.t)
     (d : nat)
   : imp (result ParallelLoop.t) :=
   BIND pol' <- phase_pipeline_opt_prepared_from_poly_no_iss_poly pol -;
+  checked_parallel_current_annotated_codegen_at pol' d.
+
+Definition parallel_current_diamond_prepared_from_poly
+    (pol : PolyLang.t)
+    (d : nat)
+  : imp (result ParallelLoop.t) :=
+  BIND pol' <- diamond_phase_pipeline_opt_prepared_from_poly_no_iss_poly pol -;
   checked_parallel_current_annotated_codegen_at pol' d.
 
 Definition parallel_current_identity_prepared_from_poly_with_iss
@@ -234,6 +327,15 @@ Definition opt_parallel_current
   BIND pol0 <- res_to_alarm PolyLang.dummy (CoreOpt.Extractor.extractor loop) -;
   let pol := CoreOpt.Strengthen.strengthen_pprog pol0 in
   BIND res <- parallel_current_prepared_from_poly pol d -;
+  res_to_alarm parallel_dummy res.
+
+Definition opt_parallel_current_diamond
+    (loop : LoopIR.t)
+    (d : nat)
+  : imp ParallelLoop.t :=
+  BIND pol0 <- res_to_alarm PolyLang.dummy (CoreOpt.Extractor.extractor loop) -;
+  let pol := CoreOpt.Strengthen.strengthen_pprog pol0 in
+  BIND res <- parallel_current_diamond_prepared_from_poly pol d -;
   res_to_alarm parallel_dummy res.
 
 Definition opt_parallel_current_identity_with_iss
