driver/ParallelPolOptCorrect.v
@@ -6,6 +6,7 @@ Require Import PolIRs.
 Require Import PolOpt.
 Require Import ParallelPolOpt.
 Require Import Result.
+Require Import List.
 
 Local Open Scope impure_scope.
 
@@ -194,6 +195,380 @@ Proof.
          pol_source pol_out Hwf_source pol_out Hopt eq_refl)
       as Hwf_out.
     eapply PolyLang.wf_pprog_affine_implies_wf_pprog_general; eauto.
+Qed.
+
+Lemma try_verified_diamond_after_phase_mid_poly_correct :
+  forall pol_mid mid_scop posttile_scop after_scop pol_out st st',
+    PolyLang.wf_pprog_affine pol_mid ->
+    mayReturn
+      (Core.try_verified_diamond_after_phase_mid_poly
+         pol_mid mid_scop posttile_scop after_scop)
+      pol_out ->
+    PolyLang.instance_list_semantics pol_out st st' ->
+    exists st'',
+      PolyLang.instance_list_semantics pol_mid st st'' /\ State.eq st' st''.
+Proof.
+  intros pol_mid mid_scop posttile_scop after_scop pol_out st st'
+         Hwf_mid Hopt Hsem_out.
+  unfold Core.try_verified_diamond_after_phase_mid_poly in Hopt.
+  destruct (Core.CoreOpt.infer_tiling_witness_scops mid_scop posttile_scop)
+    as [ws|msg] eqn:Hws.
+  - destruct
+      (Core.ValidatorCore.import_canonical_tiled_after_poly pol_mid posttile_scop ws)
+      as [pol_posttile|msg_after] eqn:Hposttile.
+    + bind_imp_destruct Hopt ok_shape Hcheck_shape.
+      destruct ok_shape.
+      * destruct (Core.TilingSched.infer_pprog_tiling_bands
+                    (Core.TilingSched.Base.outer_to_tiling_pprog pol_mid) ws)
+          as [bands|] eqn:Hbands.
+        -- bind_imp_destruct Hopt ok_perm Hcheck_perm.
+           destruct ok_perm.
+           ++ bind_imp_destruct Hopt wf_posttile_ok Hwf_posttile_check.
+              destruct wf_posttile_ok.
+              ** destruct (PolyLang.from_openscop_schedule_only
+                             pol_posttile after_scop)
+                   as [pol_after|msg_final] eqn:Hafter.
+                 --- bind_imp_destruct Hopt final_ok Hfinal.
+                     destruct final_ok.
+                     +++ bind_imp_destruct Hopt wf_after_ok Hwf_check.
+                         destruct wf_after_ok.
+                         *** apply mayReturn_pure in Hopt.
+                             subst pol_out.
+                             pose proof
+                               (Core.ValidatorCore.check_wf_polyprog_general_correct
+                                  pol_after true Hwf_check eq_refl)
+                               as Hwf_after.
+                             pose proof
+                               (proj1
+                                  (PolyLang.instance_list_semantics_current_view_iff
+                                     pol_after st st' Hwf_after)
+                                  Hsem_out)
+                               as Hsem_after.
+                             pose proof
+                               (Core.ValidatorCore.validate_general_correct
+                                  pol_posttile pol_after st st'
+                                  true Hfinal eq_refl Hsem_after)
+                               as Hfinal_corr.
+                             destruct Hfinal_corr as [st_post [Hpost_sem Heq_post]].
+                             remember (Core.TilingSched.Base.outer_to_tiling_pprog pol_mid)
+                               as before_tiling eqn:Hbefore_tiling_eq.
+                             remember (Core.TilingSched.Base.outer_to_tiling_pprog pol_posttile)
+                               as after_tiling eqn:Hafter_tiling_eq.
+                             pose proof Hcheck_shape as Hcheck_shape_sched.
+                             unfold Core.TilingSched.checked_tiling_schedule_stripmined_validate_poly,
+                                    Core.TilingSched.checked_tiling_schedule_stripmined_validate_outer
+                               in Hcheck_shape.
+                             unfold Core.TilingSched.checked_tiling_schedule_stripmined_validate_poly,
+                                    Core.TilingSched.checked_tiling_schedule_stripmined_validate_outer,
+                                    Core.TilingSched.checked_tiling_schedule_stripmined_validate
+                               in Hcheck_shape_sched.
+                             apply mayReturn_pure in Hcheck_shape_sched.
+                             apply andb_true_iff in Hcheck_shape_sched.
+                             destruct Hcheck_shape_sched as [_ Hsched_only].
+                             destruct before_tiling as [[before_pis before_ctxt] before_vars].
+                             destruct after_tiling as [[after_pis after_ctxt] after_vars].
+                             simpl in Hbefore_tiling_eq, Hafter_tiling_eq.
+                             rewrite <- Hbefore_tiling_eq in Hcheck_shape, Hsched_only.
+                             rewrite <- Hafter_tiling_eq in Hcheck_shape, Hsched_only.
+                             simpl in Hcheck_shape, Hsched_only, Hbands.
+                             pose proof
+                               (Core.TilingSched.check_pprog_tiling_schedule_stripminedb_ctxt_sound
+                                  (before_pis, before_ctxt, before_vars)
+                                  (after_pis, after_ctxt, after_vars)
+                                  ws Hsched_only)
+                               as [Hctxt_eq Hvars_eq].
+                             pose proof
+                               (Core.TilingSched.Base.outer_to_tiling_wf_pprog_affine
+                                  pol_mid Hwf_mid)
+                               as Hwf_before_tiling.
+                             rewrite <- Hbefore_tiling_eq in Hwf_before_tiling.
+                             destruct Hwf_before_tiling as [_ Hwf_before_tiling].
+                             assert (Hwfbefore_pis :
+                               List.Forall
+                                 (Core.TilingSched.Base.Tiling.PL.wf_pinstr_tiling
+                                    before_ctxt before_vars)
+                                 before_pis).
+                             {
+                               eapply List.Forall_forall.
+                               intros pi Hin.
+                               eapply
+                                 Core.TilingSched.Base.Tiling.PL.wf_pinstr_affine_implies_wf_pinstr_tiling.
+                               eapply Hwf_before_tiling; eauto.
+                             }
+                             pose proof
+                               (Core.ValidatorCore.check_wf_polyprog_general_correct
+                                  pol_posttile true Hwf_posttile_check eq_refl)
+                               as Hwf_posttile.
+                             pose proof
+                               (Core.TilingSched.Base.outer_to_tiling_wf_pprog_general
+                                  pol_posttile Hwf_posttile)
+                               as Hwf_after_tiling.
+                             rewrite <- Hafter_tiling_eq in Hwf_after_tiling.
+                             rewrite <- Hctxt_eq, <- Hvars_eq in Hwf_after_tiling.
+                             destruct Hwf_after_tiling as [_ Hwf_after_tiling].
+                             assert (Hwfafter_pis :
+                               List.Forall
+                                 (Core.TilingSched.Base.Tiling.PL.wf_pinstr_tiling
+                                    before_ctxt before_vars)
+                                 after_pis).
+                             {
+                               eapply List.Forall_forall.
+                               intros pi Hin.
+                               eapply Hwf_after_tiling; eauto.
+                             }
+                             rewrite <- Hctxt_eq, <- Hvars_eq in Hcheck_shape, Hcheck_perm.
+                             pose proof
+                               (Core.TilingSched.checked_tiling_schedule_stripmined_and_band_validate_correct_same_ctxt
+                                  before_pis before_ctxt before_vars
+                                  after_pis
+                                  ws bands st st_post
+                                  Hcheck_shape Hbands
+                                  Hwfbefore_pis Hwfafter_pis
+                                  Hcheck_perm)
+                               as Hcorr.
+                             apply Core.TilingSched.Base.outer_to_tiling_instance_list_semantics_iff
+                               in Hpost_sem.
+                             rewrite <- Hafter_tiling_eq in Hpost_sem.
+                             rewrite <- Hctxt_eq, <- Hvars_eq in Hpost_sem.
+                             specialize (Hcorr Hpost_sem).
+                             destruct Hcorr as [st_mid [Hmid_tiling Heq_mid]].
+                             rewrite Hbefore_tiling_eq in Hmid_tiling.
+                             apply Core.TilingSched.Base.outer_to_tiling_instance_list_semantics_iff
+                               in Hmid_tiling.
+                             exists st_mid.
+                             split; auto.
+                             eapply State.eq_trans; eauto.
+                         *** apply mayReturn_pure in Hopt.
+                             subst pol_out.
+                             exists st'. split; auto. eapply State.eq_refl.
+                     +++ apply mayReturn_pure in Hopt.
+                         subst pol_out.
+                         exists st'. split; auto. eapply State.eq_refl.
+                 --- apply mayReturn_pure in Hopt.
+                     subst pol_out.
+                     exists st'. split; auto. eapply State.eq_refl.
+              ** apply mayReturn_pure in Hopt.
+                 subst pol_out.
+                 exists st'. split; auto. eapply State.eq_refl.
+           ++ apply mayReturn_pure in Hopt.
+              subst pol_out.
+              exists st'. split; auto. eapply State.eq_refl.
+        -- apply mayReturn_pure in Hopt.
+           subst pol_out.
+           exists st'. split; auto. eapply State.eq_refl.
+      * apply mayReturn_pure in Hopt.
+        subst pol_out.
+        exists st'. split; auto. eapply State.eq_refl.
+    + apply mayReturn_pure in Hopt.
+      subst pol_out.
+      exists st'. split; auto. eapply State.eq_refl.
+  - apply mayReturn_pure in Hopt.
+    subst pol_out.
+    exists st'. split; auto. eapply State.eq_refl.
+Qed.
+
+Lemma try_verified_diamond_after_phase_mid_poly_wf :
+  forall pol_mid mid_scop posttile_scop after_scop pol_out,
+    PolyLang.wf_pprog_affine pol_mid ->
+    mayReturn
+      (Core.try_verified_diamond_after_phase_mid_poly
+         pol_mid mid_scop posttile_scop after_scop)
+      pol_out ->
+    PolyLang.wf_pprog_general pol_out.
+Proof.
+  intros pol_mid mid_scop posttile_scop after_scop pol_out Hwf_mid Hopt.
+  unfold Core.try_verified_diamond_after_phase_mid_poly in Hopt.
+  destruct (Core.CoreOpt.infer_tiling_witness_scops mid_scop posttile_scop)
+    as [ws|msg] eqn:Hws.
+  - destruct
+      (Core.ValidatorCore.import_canonical_tiled_after_poly pol_mid posttile_scop ws)
+      as [pol_posttile|msg_after] eqn:Hposttile.
+    + bind_imp_destruct Hopt ok_shape Hcheck_shape.
+      destruct ok_shape.
+      * destruct (Core.TilingSched.infer_pprog_tiling_bands
+                    (Core.TilingSched.Base.outer_to_tiling_pprog pol_mid) ws)
+          as [bands|] eqn:Hbands.
+        -- bind_imp_destruct Hopt ok_perm Hcheck_perm.
+           destruct ok_perm.
+           ++ bind_imp_destruct Hopt wf_posttile_ok Hwf_posttile_check.
+              destruct wf_posttile_ok.
+              ** destruct (PolyLang.from_openscop_schedule_only
+                             pol_posttile after_scop)
+                   as [pol_after|msg_final] eqn:Hafter.
+                 --- bind_imp_destruct Hopt final_ok Hfinal.
+                     destruct final_ok.
+                     +++ bind_imp_destruct Hopt wf_after_ok Hwf_check.
+                         destruct wf_after_ok.
+                         *** apply mayReturn_pure in Hopt.
+                             subst pol_out.
+                             pose proof
+                               (Core.ValidatorCore.check_wf_polyprog_general_correct
+                                  pol_after true Hwf_check eq_refl)
+                               as Hwf_after.
+                             pose proof
+                               (PolyLang.wf_pprog_general_current_view_affine
+                                  pol_after Hwf_after)
+                               as Hwf_cur_aff.
+                             eapply PolyLang.wf_pprog_affine_implies_wf_pprog_general; eauto.
+                         *** apply mayReturn_pure in Hopt.
+                             subst pol_out.
+                             eapply PolyLang.wf_pprog_affine_implies_wf_pprog_general; eauto.
+                     +++ apply mayReturn_pure in Hopt.
+                         subst pol_out.
+                         eapply PolyLang.wf_pprog_affine_implies_wf_pprog_general; eauto.
+                 --- apply mayReturn_pure in Hopt.
+                     subst pol_out.
+                     eapply PolyLang.wf_pprog_affine_implies_wf_pprog_general; eauto.
+              ** apply mayReturn_pure in Hopt.
+                 subst pol_out.
+                 eapply PolyLang.wf_pprog_affine_implies_wf_pprog_general; eauto.
+           ++ apply mayReturn_pure in Hopt.
+              subst pol_out.
+              eapply PolyLang.wf_pprog_affine_implies_wf_pprog_general; eauto.
+        -- apply mayReturn_pure in Hopt.
+           subst pol_out.
+           eapply PolyLang.wf_pprog_affine_implies_wf_pprog_general; eauto.
+      * apply mayReturn_pure in Hopt.
+        subst pol_out.
+        eapply PolyLang.wf_pprog_affine_implies_wf_pprog_general; eauto.
+    + apply mayReturn_pure in Hopt.
+      subst pol_out.
+      eapply PolyLang.wf_pprog_affine_implies_wf_pprog_general; eauto.
+  - apply mayReturn_pure in Hopt.
+    subst pol_out.
+    eapply PolyLang.wf_pprog_affine_implies_wf_pprog_general; eauto.
+Qed.
+
+Lemma try_diamond_phase_pipeline_from_source_pol_poly_correct :
+  forall pol_source before_scop pol_out st st',
+    PolyLang.wf_pprog_affine pol_source ->
+    mayReturn
+      (Core.try_diamond_phase_pipeline_from_source_pol_poly
+         pol_source before_scop)
+      pol_out ->
+    PolyLang.instance_list_semantics pol_out st st' ->
+    exists st'',
+      PolyLang.instance_list_semantics pol_source st st'' /\ State.eq st' st''.
+Proof.
+  intros pol_source before_scop pol_out st st'
+         Hwf_source Hopt Hsem_out.
+  unfold Core.try_diamond_phase_pipeline_from_source_pol_poly in Hopt.
+  destruct (Core.CoreOpt.run_pluto_diamond_phase_pipeline before_scop)
+    as [[mid_scop [posttile_scop after_scop]]|msg] eqn:Hphase.
+  - destruct (Core.PolyLang.from_openscop_like_source pol_source mid_scop)
+      as [pol_mid|msg_mid] eqn:Hmid.
+    + bind_imp_destruct Hopt affine_ok Haff.
+      destruct affine_ok.
+      * pose proof
+          (Core.ValidatorCore.validate_preserve_wf_pprog
+             pol_source pol_mid _ Haff eq_refl)
+          as [_ Hwf_mid].
+        pose proof
+          (try_verified_diamond_after_phase_mid_poly_correct
+             pol_mid mid_scop posttile_scop after_scop pol_out st st'
+             Hwf_mid Hopt Hsem_out)
+          as Hmid_corr.
+        destruct Hmid_corr as [st_mid [Hmid_sem Heq_mid]].
+        pose proof
+          (Core.ValidatorCore.validate_correct
+             pol_source pol_mid st st_mid true Haff eq_refl Hmid_sem)
+          as Haff_corr.
+        destruct Haff_corr as [st_src [Hsrc_sem Heq_src]].
+        exists st_src.
+        split; auto.
+        eapply State.eq_trans; eauto.
+      * eapply CoreOpt.scheduler'_correct; eauto.
+    + eapply CoreOpt.scheduler'_correct; eauto.
+  - eapply CoreOpt.scheduler'_correct; eauto.
+Qed.
+
+Lemma try_diamond_phase_pipeline_from_source_pol_poly_wf :
+  forall pol_source before_scop pol_out,
+    PolyLang.wf_pprog_affine pol_source ->
+    mayReturn
+      (Core.try_diamond_phase_pipeline_from_source_pol_poly
+         pol_source before_scop)
+      pol_out ->
+    PolyLang.wf_pprog_general pol_out.
+Proof.
+  intros pol_source before_scop pol_out Hwf_source Hopt.
+  unfold Core.try_diamond_phase_pipeline_from_source_pol_poly in Hopt.
+  destruct (Core.CoreOpt.run_pluto_diamond_phase_pipeline before_scop)
+    as [[mid_scop [posttile_scop after_scop]]|msg] eqn:Hphase.
+  - destruct (Core.PolyLang.from_openscop_like_source pol_source mid_scop)
+      as [pol_mid|msg_mid] eqn:Hmid.
+    + bind_imp_destruct Hopt affine_ok Haff.
+      destruct affine_ok.
+      * pose proof
+          (Core.ValidatorCore.validate_preserve_wf_pprog
+             pol_source pol_mid _ Haff eq_refl)
+          as [_ Hwf_mid].
+        eapply try_verified_diamond_after_phase_mid_poly_wf; eauto.
+      * pose proof
+          (CoreOpt.scheduler'_preserve_wf
+             pol_source pol_out Hwf_source pol_out Hopt eq_refl)
+          as Hwf_out.
+        eapply PolyLang.wf_pprog_affine_implies_wf_pprog_general; eauto.
+    + pose proof
+        (CoreOpt.scheduler'_preserve_wf
+           pol_source pol_out Hwf_source pol_out Hopt eq_refl)
+        as Hwf_out.
+      eapply PolyLang.wf_pprog_affine_implies_wf_pprog_general; eauto.
+  - pose proof
+      (CoreOpt.scheduler'_preserve_wf
+         pol_source pol_out Hwf_source pol_out Hopt eq_refl)
+      as Hwf_out.
+    eapply PolyLang.wf_pprog_affine_implies_wf_pprog_general; eauto.
+Qed.
+
+Lemma diamond_phase_pipeline_opt_prepared_from_poly_no_iss_poly_correct :
+  forall pol pol_out st st',
+    PolyLang.wf_pprog_affine pol ->
+    mayReturn (Core.diamond_phase_pipeline_opt_prepared_from_poly_no_iss_poly pol) pol_out ->
+    PolyLang.instance_list_semantics pol_out st st' ->
+    exists st'',
+      PolyLang.instance_list_semantics pol st st'' /\ State.eq st' st''.
+Proof.
+  intros pol pol_out st st' Hwf Hopt Hsem_out.
+  unfold Core.diamond_phase_pipeline_opt_prepared_from_poly_no_iss_poly in Hopt.
+  destruct (Core.CoreOpt.has_nonscalar_stmt pol) eqn:Hnonscalar.
+  { destruct (Core.CoreOpt.export_for_phase_scheduler pol) as [before_scop|] eqn:Hbefore.
+    { simpl in Hopt.
+      eapply try_diamond_phase_pipeline_from_source_pol_poly_correct.
+      - exact Hwf.
+      - exact Hopt.
+      - exact Hsem_out. }
+    { simpl in Hopt.
+      eapply CoreOpt.scheduler'_correct.
+      - exact Hopt.
+      - exact Hsem_out. } }
+  { simpl in Hopt.
+    eapply mayReturn_pure in Hopt. subst pol_out.
+    exists st'. split; auto. eapply State.eq_refl. }
+Qed.
+
+Lemma diamond_phase_pipeline_opt_prepared_from_poly_no_iss_poly_wf :
+  forall pol pol_out,
+    PolyLang.wf_pprog_affine pol ->
+    mayReturn (Core.diamond_phase_pipeline_opt_prepared_from_poly_no_iss_poly pol) pol_out ->
+    PolyLang.wf_pprog_general pol_out.
+Proof.
+  intros pol pol_out Hwf Hopt.
+  unfold Core.diamond_phase_pipeline_opt_prepared_from_poly_no_iss_poly in Hopt.
+  destruct (Core.CoreOpt.has_nonscalar_stmt pol) eqn:Hnonscalar.
+  { destruct (Core.CoreOpt.export_for_phase_scheduler pol) as [before_scop|] eqn:Hbefore.
+    { simpl in Hopt.
+      eapply try_diamond_phase_pipeline_from_source_pol_poly_wf.
+      - exact Hwf.
+      - exact Hopt. }
+    { simpl in Hopt.
+      pose proof
+        (CoreOpt.scheduler'_preserve_wf pol pol_out Hwf pol_out Hopt eq_refl)
+        as Hwf_out.
+      eapply PolyLang.wf_pprog_affine_implies_wf_pprog_general; eauto. } }
+  { simpl in Hopt.
+    eapply mayReturn_pure in Hopt. subst pol_out.
+    eapply PolyLang.wf_pprog_affine_implies_wf_pprog_general; eauto. }
 Qed.
 
 Lemma phase_pipeline_opt_prepared_from_poly_no_iss_poly_correct :
@@ -544,6 +919,36 @@ Proof.
   eapply State.eq_trans; eauto.
 Qed.
 
+Lemma parallel_current_diamond_prepared_from_poly_correct :
+  forall pol d pl st st',
+    PolyLang.wf_pprog_affine pol ->
+    mayReturn (Core.parallel_current_diamond_prepared_from_poly pol d) (Okk pl) ->
+    ParallelLoop.semantics pl st st' ->
+    exists st'',
+      PolyLang.instance_list_semantics pol st st'' /\ State.eq st' st''.
+Proof.
+  intros pol d pl st st' Hwf Hopt Hsem.
+  unfold Core.parallel_current_diamond_prepared_from_poly in Hopt.
+  bind_imp_destruct Hopt pol_after Hdiamond.
+  pose proof
+    (diamond_phase_pipeline_opt_prepared_from_poly_no_iss_poly_wf
+       pol pol_after Hwf Hdiamond)
+    as Hwf_after.
+  pose proof
+    (checked_parallel_current_annotated_codegen_at_correct
+       pol_after d pl st st' Hopt Hwf_after Hsem)
+    as Hafter_corr.
+  destruct Hafter_corr as [st_after [Hafter_sem Heq_after]].
+  pose proof
+    (diamond_phase_pipeline_opt_prepared_from_poly_no_iss_poly_correct
+       pol pol_after st st_after Hwf Hdiamond Hafter_sem)
+    as Hdiamond_corr.
+  destruct Hdiamond_corr as [st_src [Hsrc_sem Heq_src]].
+  exists st_src.
+  split; auto.
+  eapply State.eq_trans; eauto.
+Qed.
+
 Lemma parallel_current_identity_prepared_from_poly_with_iss_correct :
   forall pol d pl st st',
     PolyLang.wf_pprog_affine pol ->
@@ -736,6 +1141,40 @@ Proof.
   - exact Heq_src.
 Qed.
 
+Theorem Opt_parallel_current_diamond_result_correct :
+  forall loop d pl st st',
+    mayReturn (Core.Opt_parallel_current_diamond_result loop d) (Okk pl) ->
+    ParallelLoop.semantics pl st st' ->
+    exists st'',
+      LoopIR.semantics loop st st'' /\ State.eq st' st''.
+Proof.
+  intros loop d pl st st' Hopt Hsem.
+  unfold Core.Opt_parallel_current_diamond_result in Hopt.
+  bind_imp_destruct Hopt pol0 Hextimp.
+  set (pol := CoreOpt.Strengthen.strengthen_pprog pol0) in *.
+  pose proof Hextimp as Hextok.
+  apply res_to_alarm_correct in Hextok.
+  pose proof
+    (CoreOpt.Strengthen.strengthen_pprog_wf_affine
+       pol0
+       (CoreOpt.extractor_success_wf_pprog_affine loop pol0 Hextok))
+    as Hwf_pol.
+  pose proof
+    (parallel_current_diamond_prepared_from_poly_correct
+       pol d pl st st' Hwf_pol Hopt Hsem)
+    as Hphase_corr.
+  destruct Hphase_corr as [st_str [Hstr_sem Heq_str]].
+  eapply CoreOpt.Strengthen.instance_list_semantics_unstrengthen in Hstr_sem.
+  pose proof (CoreOpt.Extractor.extractor_correct loop pol0 st st_str Hextok Hstr_sem)
+    as Hext_corr.
+  destruct Hext_corr as [st_src [Hloop_src Heq_src]].
+  exists st_src.
+  split; auto.
+  eapply State.eq_trans.
+  - exact Heq_str.
+  - exact Heq_src.
+Qed.
+
 Theorem Opt_parallel_current_identity_with_iss_result_correct :
   forall loop d pl st st',
     mayReturn (Core.Opt_parallel_current_identity_with_iss_result loop d) (Okk pl) ->
@@ -884,6 +1323,22 @@ Proof.
   apply res_to_alarm_correct in Hopt_ok.
   subst res.
   eapply Opt_parallel_current_result_correct; eauto.
+Qed.
+
+Theorem Opt_parallel_current_diamond_correct :
+  forall loop d pl st st',
+    mayReturn (Core.Opt_parallel_current_diamond loop d) pl ->
+    ParallelLoop.semantics pl st st' ->
+    exists st'',
+      LoopIR.semantics loop st st'' /\ State.eq st' st''.
+Proof.
+  intros loop d pl st st' Hopt Hsem.
+  unfold Core.Opt_parallel_current_diamond in Hopt.
+  bind_imp_destruct Hopt res Hres.
+  pose proof Hopt as Hopt_ok.
+  apply res_to_alarm_correct in Hopt_ok.
+  subst res.
+  eapply Opt_parallel_current_diamond_result_correct; eauto.
 Qed.
 
 Theorem Opt_parallel_current_identity_with_iss_correct :
